Tests/Examples/Lambda.lean
@@ -4,36 +4,36 @@ import Tests.Basic
 open Parser Term
 
 -- variable
-#guard term.runResult? (toText "x") == some (.var "x")
+#guard term.runOption "x" == some (.var "x")
 
 -- lambda
-#guard term.runResult? (toText "\\x. x") == some (.lam "x" (.var "x"))
+#guard term.runOption "\\x. x" == some (.lam "x" (.var "x"))
 
 -- application
-#guard term.runResult? (toText "f x") == some (.app (.var "f") (.var "x"))
+#guard term.runOption "f x" == some (.app (.var "f") (.var "x"))
 
 -- left-associative application
-#guard term.runResult? (toText "f x y")
+#guard term.runOption "f x y"
     == some (.app (.app (.var "f") (.var "x")) (.var "y"))
 
 -- nested lambda
-#guard term.runResult? (toText "\\x. \\y. x")
+#guard term.runOption "\\x. \\y. x"
     == some (.lam "x" (.lam "y" (.var "x")))
 
 -- lambda body extends right
-#guard term.runResult? (toText "\\f. f x")
+#guard term.runOption "\\f. f x"
     == some (.lam "f" (.app (.var "f") (.var "x")))
 
 -- parenthesized lambda in application
-#guard term.runResult? (toText "(\\x. x) y")
+#guard term.runOption "(\\x. x) y"
     == some (.app (.lam "x" (.var "x")) (.var "y"))
 
 -- church numeral
-#guard term.runResult? (toText "\\f. \\x. f (f x)")
+#guard term.runOption "\\f. \\x. f (f x)"
     == some (.lam "f" (.lam "x" (.app (.var "f") (.app (.var "f") (.var "x")))))
 
 -- negative: empty
-#guard term.runResult? (toText "") == none
+#guard term.runOption "" == none
 
 -- negative: lone backslash
-#guard term.runResult? (toText "\\") == none
+#guard term.runOption "\\" == none
