Tests/Examples/SExp.lean
@@ -3,12 +3,12 @@ import Tests.Basic
 
 open Parser SExp
 
-#guard sexp.runResult? (toText "hello") == some (.atom "hello")
+#guard sexp.runOption "hello" == some (.atom "hello")
 
-#guard sexp.runResult? (toText "(a b)") == some (.pair (.atom "a") (.atom "b"))
+#guard sexp.runOption "(a b)" == some (.pair (.atom "a") (.atom "b"))
 
-#guard sexp.runResult? (toText "(a b c)")
+#guard sexp.runOption "(a b c)"
     == some (.pair (.atom "a") (.pair (.atom "b") (.atom "c")))
 
-#guard sexp.runResult? (toText "(a (b c))")
+#guard sexp.runOption "(a (b c))"
     == some (.pair (.atom "a") (.pair (.atom "b") (.atom "c")))
